Nearly completed with revising the Heap definition

Heap.v
@@ -1,14 +1,18 @@
-Require Import Fiat.ADT Fiat.ADTNotation.
+Require Import
+  Coq.Sets.Ensembles
+  Coq.NArith.NArith
+  Omega.
 
-Require Import Coq.Sets.Ensembles.
-Require Import Coq.NArith.NArith.
+Require Import
+  Fiat.ADT
+  Fiat.ADTNotation
+  Here.ADTInduction
+  Here.LibExt
+  Here.Decidable.
 
-Require Import Here.ADTInduction.
-Require Import Here.LibExt.
-Require Import Here.Decidable.
+Generalizable All Variables.
 
 Open Scope string_scope.
-Open Scope N_scope.
 
 Definition emptyS   := "empty".
 Definition allocS   := "alloc".
@@ -23,203 +27,555 @@ Section Heap.
 
 Variable Word8 : Type.
 
+Open Scope N_scope.
+
 Definition within (addr : N) (len : N) (a : N) : Prop :=
   addr <= a < addr + len.
 
 Definition within_le (addr : N) (len : N) (a : N) : Prop :=
   addr <= a <= addr + len.
 
-Definition fits (addr len addr2 len2 : N) : Prop :=
-  within addr len addr2 /\ within_le addr len (addr2 + len2).
+Definition fits (addr len off sz : N) : Prop :=
+  within addr len off /\ off + sz <= len.
 
 Definition overlaps (addr len addr2 len2 : N) : Prop :=
   addr < addr2 + len2 /\ addr2 < addr + len.
 
-Definition HeapSpec := Def ADT {
-  (* a set of addr + len pairs to mark allocations,
-     and another set to locate bytes *)
-  rep := Ensemble (N * N) * Ensemble (N * Word8),
+Lemma overlaps_sym : forall addr1 len1 addr2 len2,
+  overlaps addr1 len1 addr2 len2 <-> overlaps addr2 len2 addr1 len1.
+Proof.
+  unfold overlaps; split; intros;
+  destruct H; split; trivial.
+Qed.
 
-  Def Constructor0 emptyS : rep := ret (Empty_set _, Empty_set _),,
+Lemma overlaps_irr : forall addr len1 len2,
+  0 < len1 -> 0 < len2 -> overlaps addr len1 addr len2.
+Proof.
+  unfold overlaps; split; intros;
+  apply N.lt_add_pos_r; assumption.
+Qed.
+
+Record MemoryBlock := {
+  memAddr : N;
+  memSize : N;
+  memData : Ensemble (N * Word8)
+}.
+
+Record CorrectMemoryBlock (blk : MemoryBlock) : Prop := {
+  _ : 0 < memSize blk;
+  _ : forall off val,
+        In _ (memData blk) (off, val) -> off < memSize blk;
+  _ : forall off val1 val2,
+        In _ (memData blk) (off, val1) ->
+        In _ (memData blk) (off, val2) -> val1 = val2
+}.
+
+Definition CorrectHeap (mem : Ensemble MemoryBlock) : Prop :=
+  forall blk, mem ↝ blk -> CorrectMemoryBlock blk.
+
+Definition shift_address (addr1 addr2 : N) (mem : Ensemble MemoryBlock) :
+  Ensemble MemoryBlock :=
+  blk <- mem;
+  ret {| memAddr := IfDec addr1 = memAddr blk
+                    Then addr2
+                    Else memAddr blk
+       ; memSize := memSize blk
+       ; memData := memData blk |}.
+
+Lemma shift_address_correct `(_ : CorrectHeap mem) :
+  forall addr1 addr2 blk', shift_address addr1 addr2 mem ↝ blk'
+    -> CorrectMemoryBlock blk'.
+Proof.
+  unfold CorrectHeap in CorrectHeap0.
+  unfold shift_address, IfDec_Then_Else; simpl.
+  intros.
+  simplify_ensembles; subst.
+  destruct (CorrectHeap0 x H).
+  constructor; simpl in *; intros; eauto.
+Qed.
+
+Definition fit_to_length (addr : N) (len : N | 0 < len)
+           (mem : Ensemble MemoryBlock) :
+  Ensemble MemoryBlock :=
+  blk <- mem;
+  ret (IfDec addr = memAddr blk
+       Then {| memAddr := memAddr blk
+             ; memSize := proj1_sig len
+             ; memData := fun p => fst p < proj1_sig len /\ memData blk p |}
+       Else blk).
+
+Lemma fit_to_length_correct `(_ : CorrectHeap mem) :
+  forall addr len blk', fit_to_length addr len mem ↝ blk'
+    -> CorrectMemoryBlock blk'.
+Proof.
+  unfold CorrectHeap in CorrectHeap0.
+  unfold fit_to_length, IfDec_Then_Else; simpl.
+  intros.
+  simplify_ensembles.
+  pose proof (CorrectHeap0 x H).
+  destruct (addr =? memAddr x);
+  [| subst; assumption ].
+  destruct H1; clear H1 H2.
+  simplify_ensembles; subst; simpl.
+  destruct len; simpl.
+  constructor; simpl in *; intros; trivial;
+  unfold Ensembles.In in *; simpl in *; intuition.
+  apply (H3 off val1 val2); assumption.
+Qed.
+
+Definition set_address (addr : N) (x : Word8) (mem : Ensemble MemoryBlock) :
+  Comp (MemoryBlock * bool) :=
+  blk <- mem;
+  ret (IfDec within (memAddr blk) (memSize blk) addr
+       Then ({| memAddr := memAddr blk
+              ; memSize := memSize blk
+              ; memData :=
+                  let off := addr - memAddr blk in
+                  Add _ (Setminus _  (memData blk) (fun p => fst p = off))
+                        (off, x) |}, true)
+       Else (blk, false)).
+
+Lemma set_address_correct `(_ : CorrectHeap mem) :
+  forall addr x blk' b, set_address addr x mem ↝ (blk', b)
+    -> CorrectMemoryBlock blk'.
+Proof.
+  unfold CorrectHeap in CorrectHeap0.
+  unfold set_address, IfDec_Then_Else; simpl.
+  intros.
+  simplify_ensembles.
+  pose proof (CorrectHeap0 x0 H).
+  destruct ((memAddr x0 <=? addr) &&
+            (addr <? memAddr x0 + memSize x0))%bool eqn:Heqe; inv H0;
+  [| assumption ].
+  destruct H1.
+  constructor; simpl; intros; trivial.
+  - inv H3; inv H4.
+      apply (H1 off val); assumption.
+    apply Bool.andb_true_iff in Heqe; destruct Heqe.
+    apply N.leb_le in H3.
+    rewrite N2Z.inj_lt, N2Z.inj_sub; trivial.
+    rewrite N2Z.inj_le in H3.
+    apply N.ltb_lt in H4.
+    rewrite N2Z.inj_lt, N2Z.inj_add in H4.
+    omega.
+  - inv H3; inv H4; inv H3; inv H5.
+    + apply (H2 off); assumption.
+    + contradiction H4; constructor.
+    + contradiction H6; constructor.
+    + reflexivity.
+Qed.
+
+Definition copy_memory
+           (addr1 addr2 : N) (len : N | 0 < len)
+           (mem : Ensemble MemoryBlock) : Comp (MemoryBlock * bool) :=
+  dst <- mem;
+  IfDec fits (memAddr dst) (memSize dst) addr2 (proj1_sig len)
+  Then (
+    src <- mem;
+    ret (IfDec fits (memAddr src) (memSize src) addr1 (proj1_sig len)
+         Then ({| memAddr := memAddr dst
+                ; memSize := memSize dst
+                ; memData :=
+                    fun p =>
+                      IfDec within addr2 (proj1_sig len) (fst p)
+                      Then memData src (addr2 + (fst p - addr1), snd p)
+                      Else memData dst p |}, true)
+         Else (dst, false))
+  )
+  Else ret (dst, false).
+
+Lemma copy_memory_correct `(_ : CorrectHeap mem) :
+  forall addr1 addr2 len blk' b, copy_memory addr1 addr2 len mem ↝ (blk', b)
+    -> CorrectMemoryBlock blk'.
+Proof.
+  unfold CorrectHeap in CorrectHeap0.
+  unfold copy_memory, IfDec_Then_Else; simpl.
+  intros.
+  destruct len; simpl in *.
+  simplify_ensembles.
+  destruct (CorrectHeap0 x0 H); clear H.
+  constructor; simpl; intros; trivial.
+  - clear -H0 H1.
+    destruct ((memAddr x0 <=? addr2) &&
+              (addr2 <? memAddr x0 + memSize x0) &&
+              (addr2 + x <=? memSize x0))%bool; subst;
+    simplify_ensembles;
+    [| inv H0; trivial ].
+    destruct ((memAddr x1 <=? addr1) &&
+              (addr1 <? memAddr x1 + memSize x1) &&
+              (addr1 + x <=? memSize x1))%bool;
+    simplify_ensembles; inv H0; subst; simpl in *; trivial.
+  - clear -H0 H2 H.
+    destruct ((memAddr x0 <=? addr2) &&
+              (addr2 <? memAddr x0 + memSize x0) &&
+              (addr2 + x <=? memSize x0))%bool eqn:Heqe; subst;
+    simplify_ensembles; subst; trivial.
+      destruct ((memAddr x1 <=? addr1) &&
+                (addr1 <? memAddr x1 + memSize x1) &&
+                (addr1 + x <=? memSize x1))%bool;
+      simplify_ensembles; inv H1; subst; simpl in *.
+        unfold Ensembles.In in H; simpl in H.
+        destruct ((addr2 <=? off) && (off <? addr2 + x))%bool eqn:Heqe2.
+          apply Bool.andb_true_iff in Heqe; destruct Heqe.
+          apply Bool.andb_true_iff in Heqe2; destruct Heqe2.
+          clear -H3 H4 H5.
+          apply N.leb_le in H4.
+          apply N.leb_le in H3.
+          rewrite N2Z.inj_le, N2Z.inj_add in H3.
+          rewrite N2Z.inj_le in H4.
+          apply N.ltb_lt in H5.
+          rewrite N2Z.inj_lt, N2Z.inj_add in H5.
+          rewrite N2Z.inj_lt.
+          omega.
+        apply (H2 off val); assumption.
+      apply (H2 off val); assumption.
+    inv H0.
+    apply (H2 off val); assumption.
+  - clear -H0 H H4 H3 CorrectHeap0.
+    destruct ((memAddr x0 <=? addr2) &&
+              (addr2 <? memAddr x0 + memSize x0) &&
+              (addr2 + x <=? memSize x0))%bool; subst;
+    simplify_ensembles; subst; trivial.
+      destruct ((memAddr x1 <=? addr1) &&
+                (addr1 <? memAddr x1 + memSize x1) &&
+                (addr1 + x <=? memSize x1))%bool;
+      simplify_ensembles; inv H1; subst; simpl in *.
+      {
+        destruct (CorrectHeap0 x1 H0).
+        unfold Ensembles.In in *; simpl in *.
+        destruct ((addr2 <=? off) && (off <? addr2 + x))%bool.
+          apply (H5 (addr2 + (off - addr1)) val1 val2); assumption.
+        apply (H3 off val1 val2); assumption.
+      }
+      apply (H3 off val1 val2); assumption.
+    inv H0.
+    apply (H3 off val1 val2); assumption.
+Qed.
+
+Definition set_memory (addr : N) (len : N | 0 < len) (w : Word8)
+           (mem : Ensemble MemoryBlock) : Comp (MemoryBlock * bool) :=
+  blk <- mem;
+  ret (IfDec fits (memAddr blk) (memSize blk) addr (proj1_sig len)
+       Then ({| memAddr := memAddr blk
+              ; memSize := memSize blk
+              ; memData := fun p =>
+                             IfDec within addr (proj1_sig len) (fst p)
+                             Then snd p = w
+                             Else memData blk p |}, true)
+       Else (blk, false)).
+
+Lemma set_memory_correct `(_ : CorrectHeap mem) :
+  forall addr len w blk' b, set_memory addr len w mem ↝ (blk', b)
+    -> CorrectMemoryBlock blk'.
+Proof.
+  unfold CorrectHeap in CorrectHeap0.
+  unfold set_memory, IfDec_Then_Else; simpl.
+  intros.
+  destruct len; simpl in *.
+  simplify_ensembles.
+  destruct (CorrectHeap0 x0 H); clear H.
+  constructor; simpl; intros; trivial.
+  - clear -H0 H1.
+    destruct ((memAddr x0 <=? addr) &&
+              (addr <? memAddr x0 + memSize x0) &&
+              (addr + x <=? memSize x0))%bool; subst;
+    simplify_ensembles; inv H0; subst; simpl in *; trivial.
+  - clear -H0 H2 H.
+    destruct ((memAddr x0 <=? addr) &&
+              (addr <? memAddr x0 + memSize x0) &&
+              (addr + x <=? memSize x0))%bool eqn:Heqe; subst;
+    simplify_ensembles; inv H0; subst; simpl in *;
+    [| apply (H2 off val); assumption].
+    unfold Ensembles.In in H; simpl in H.
+    destruct ((addr <=? off) && (off <? addr + x))%bool eqn:Heqe2;
+    [| apply (H2 off val); assumption].
+    destruct H; subst.
+    apply Bool.andb_true_iff in Heqe; destruct Heqe.
+    apply Bool.andb_true_iff in Heqe2; destruct Heqe2.
+    clear -H0 H1 H3.
+    rewrite N2Z.inj_lt.
+    apply N.leb_le in H0.
+    rewrite N2Z.inj_le, N2Z.inj_add in H0.
+    apply N.leb_le in H1.
+    apply N.ltb_lt in H3.
+    rewrite N2Z.inj_lt, N2Z.inj_add in H3.
+    omega.
+  - clear -H0 H H4 H3 CorrectHeap0.
+    destruct ((memAddr x0 <=? addr) &&
+              (addr <? memAddr x0 + memSize x0) &&
+              (addr + x <=? memSize x0))%bool; subst;
+    simplify_ensembles; inv H0; subst; trivial;
+    [| apply (H3 off val1 val2); assumption ].
+    unfold Ensembles.In in *; simpl in *.
+    destruct ((addr <=? off) && (off <? addr + x))%bool;
+    [| apply (H3 off val1 val2); assumption ].
+    destruct H, H4; subst.
+    reflexivity.
+Qed.
+
+Definition found_block
+           (addr : N)
+           (addr' len' : N)
+           (data' : Ensemble (N * Word8))
+           (mem : Ensemble MemoryBlock) : Prop :=
+  In _ mem {| memAddr := addr'
+            ; memSize := len'
+            ; memData := data' |}
+  -> within addr' len' addr.
+
+Definition no_block (addr : N) (mem : Ensemble MemoryBlock) : Prop :=
+  forall addr' len' data',
+    In _ mem {| memAddr := addr'
+              ; memSize := len'
+              ; memData := data' |}
+    -> ~ within addr' len' addr.
+
+Definition HeapSpec := Def ADT {
+  (* a mapping of addr tokens to a length, and another mapping from
+     offsets within a certain block to individual bytes *)
+  rep := Ensemble MemoryBlock,
+
+  Def Constructor0 emptyS : rep := ret (Empty_set _),,
 
   Def Method1 allocS (r : rep) (len : N | 0 < len) : rep * N :=
-    (* Allocate the block *)
     addr <- { addr : N
-            | forall addr' len', In _ (fst r) (addr', len')
+            | forall addr' len' data',
+                In _ r {| memAddr := addr'
+                        ; memSize := len'
+                        ; memData := data' |}
                 -> ~ overlaps addr (proj1_sig len) addr' len' };
-    ret ((Add _ (fst r) (addr, proj1_sig len), snd r), addr),
+    ret (Add _ r {| memAddr := addr
+                  ; memSize := proj1_sig len
+                  ; memData := Empty_set _ |}, addr),
 
-  Def Method1 freeS (r : rep) (addr : N) : rep * bool :=
-    (* Does an allocated block exist at the given address? *)
-    m <- { m : option N | forall l, m = Some l -> In _ (fst r) (addr, l) };
-    (* If yes, remove it and all its associated memory; else do nothing *)
-    ret (Ifopt m as len
-         Then ((Subtract _ (fst r) (addr, len),
-                Setminus _ (snd r) (fun p => within addr len (fst p))),
-               true)
-         Else (r, false)),
+  Def Method1 freeS (r : rep) (addr : N) : rep * unit :=
+    ret (Setminus _ r (fun p => addr = memAddr p), tt),
 
   Def Method2 reallocS (r : rep) (addr : N) (len : N | 0 < len) :
     rep * N :=
-    (* Does an allocated block exist at the given address? *)
-    m <- { m : option N | forall l, m = Some l -> In _ (fst r) (addr, l) };
-    Ifopt m as olen
-    Then
-      (* Check whether to block to be reallocated would fit at its current
-         position. If so, just update the length, otherwise deallocate and
-         reallocate it, while copying its contents to the new position. *)
-      let len := proj1_sig len in
-      IfDec len <= olen
-      Then ret (((fun p =>
-                    IF fst p = addr
-                    then snd p = len
-                    else In _ (fst r) p),
-                 (fun p =>
-                    In _ (snd r) p /\
-                    ~ within (addr + len) (addr + olen) (fst p))),
-                addr)
-      Else (
-        (* Is there enough free space to allocate the new block? *)
-        naddr <- { naddr : N
-                 | forall addr' len', In _ (fst r) (addr', len')
-                     -> ~ overlaps naddr len addr' len' };
-        (* Free the old block, allocate the new one, and copy over as
-           many bytes as possible from the previous block. *)
-        ret ((Add _ (Subtract _ (fst r) (addr, olen)) (naddr, len),
-                (fun p =>
-                   IF within naddr (N.min olen len) (fst p)
-                   then IF naddr < addr
-                        then In _ (snd r) (fst p - (addr - naddr), snd p)
-                        else In _ (snd r) (fst p + (naddr - addr), snd p)
-                   else ~ within addr len (fst p) -> In _ (snd r) p)),
-             naddr)
-      )
-    Else (
-      (* Allocate a new block *)
-      addr <- { addr : N
-              | forall addr' len', In _ (fst r) (addr', len')
-                  -> ~ overlaps addr (proj1_sig len) addr' len' };
-      ret ((Add _ (fst r) (addr, proj1_sig len), snd r), addr)),
+    naddr <- { naddr : N
+             | forall addr' len' data',
+                 In _ r {| memAddr := addr'
+                         ; memSize := len'
+                         ; memData := data' |}
+                 -> IF addr = addr'
+                    then proj1_sig len < len'
+                    else ~ overlaps naddr (proj1_sig len) addr' len' };
+    ret (fit_to_length naddr len (shift_address addr naddr r),
+         naddr),
 
-  Def Method1 peekS (r : rep) (addr : N) : rep * option Word8 :=
-    (* Retrieve the word at the given location; note that since [pokeS] is the
-       only way to set memory, and it only allows setting within an allocated
-       block, we don't need to test whether the address is allocated here. *)
-    p <- { p : option Word8 | forall x, p = Some x -> In _ (snd r) (addr, x) };
+  Def Method1 peekS (r : rep) (addr : N) : rep * Word8 :=
+    p <- { p : Word8
+         | forall base len' data',
+             found_block addr base len' data' r
+             -> In _ data' (addr - base, p) };
     ret (r, p),
 
-  Def Method2 pokeS (r : rep) (addr : N) (w : Word8) : rep * unit :=
-      (* Check whether the address is within an allocated block; if so, set the
-       memory location, otherwise do nothing. *)
-    ret ((fst r, Add _ (Setminus _ (snd r) (fun p => fst p = addr))
-                       (addr, w)), tt),
+  Def Method2 pokeS (r : rep) (addr : N) (w : Word8) : rep * bool :=
+    res <- set_address addr w r;
+    ret (ret (fst res), snd res),
 
-  Def Method3 memcpyS (r : rep) (addr : N) (addr2 : N) (len : N) : rep * unit :=
-    ret ((fst r, fun p =>
-           (* If an attempt is made to access the new region, adjust it to
-              look like an access to the old location. *)
-           IF within addr2 len (fst p)
-           then IF addr < addr2
-                then In _ (snd r) (fst p - (addr2 - addr), snd p)
-                else In _ (snd r) (fst p + (addr - addr2), snd p)
-           else In _ (snd r) p),
-         tt),
+  (* A restriction is made here that data may only be copied from within one
+     allocated block to another (or within the same original block), and that
+     the region must fit within both source and destination. Otherwise, the
+     operation is a no-op. *)
+  Def Method3 memcpyS (r : rep) (addr : N) (addr2 : N) (len : N | 0 < len) :
+    rep * bool :=
+    res <- copy_memory addr addr2 len r;
+    ret (ret (fst res), snd res),
 
-  Def Method3 memsetS (r : rep) (addr : N) (len : N) (w : Word8) : rep * bool :=
-    (* Check that the memory to be set is within an allocated region. *)
-    b <- { b | decides b
-                 (exists addr' len',
-                     In _ (fst r) (addr', len') /\
-                     within_le addr' len' (addr + len)) };
-    ret (If b
-         Then
-           ((fst r,
-             fun p =>
-               (* A reference to the set region appears as though all its
-                  bytes have that value. *)
-               IF within addr len (fst p)
-               then snd p = w
-               else In _ (snd r) p), true)
-         Else (r, false))
+  Def Method3 memsetS (r : rep) (addr : N) (len : N | 0 < len) (w : Word8) :
+    rep * bool :=
+    res <- set_memory addr len w r;
+    ret (ret (fst res), snd res)
 
 }%ADTParsing.
+
+Definition alloc (r : Rep HeapSpec) (len : N | 0 < len) :
+  Comp (Rep HeapSpec * N) :=
+  Eval simpl in callMeth HeapSpec allocS r len.
+
+Definition free (r : Rep HeapSpec) (addr : N) :
+  Comp (Rep HeapSpec * unit) :=
+  Eval simpl in callMeth HeapSpec freeS r addr.
 
 Definition realloc (r : Rep HeapSpec) (addr : N) (len : N | 0 < len) :
   Comp (Rep HeapSpec * N) :=
   Eval simpl in callMeth HeapSpec reallocS r addr len.
 
-Definition peek (r : Rep HeapSpec) (addr : N) :
-  Comp (Rep HeapSpec * option Word8) :=
+Definition peek (r : Rep HeapSpec) (addr : N) : Comp (Rep HeapSpec * Word8) :=
   Eval simpl in callMeth HeapSpec peekS r addr.
 
 Definition poke (r : Rep HeapSpec) (addr : N) (w : Word8) :
-  Comp (Rep HeapSpec * unit) :=
+  Comp (Rep HeapSpec * bool) :=
   Eval simpl in callMeth HeapSpec pokeS r addr w.
 
-Definition memcpy (r : Rep HeapSpec) (addr : N) (addr2 : N) (len : N) :
-  Comp (Rep HeapSpec * unit) :=
+Definition memcpy (r : Rep HeapSpec)
+           (addr : N) (addr2 : N) (len : N | 0 < len) :
+  Comp (Rep HeapSpec * bool) :=
   Eval simpl in callMeth HeapSpec memcpyS r addr addr2 len.
 
+Definition memset (r : Rep HeapSpec)
+           (addr : N) (len : N | 0 < len) (w : Word8) :
+  Comp (Rep HeapSpec * bool) :=
+  Eval simpl in callMeth HeapSpec memsetS r addr len w.
+
+Theorem allocations_are_correction :
+  forall r : Rep HeapSpec, fromADT _ r -> CorrectHeap r.
+Proof.
+  unfold CorrectHeap; intros.
+  generalize dependent blk.
+  ADT induction r.
+  - constructor; inversion H0.
+  - destruct x; simpl in *.
+    inv H1.
+      apply IHfromADT.
+      exact H2.
+    inv H2.
+    constructor; simpl; trivial; intros; inv H1.
+  - inv H1.
+    exact (IHfromADT _ H0).
+  - exact (fit_to_length_correct (@shift_address_correct _ IHfromADT _ _) H1).
+  - destruct v; simpl in *; inv H1.
+    exact (set_address_correct IHfromADT H0).
+  - destruct v; simpl in *; inv H1.
+    exact (copy_memory_correct IHfromADT H0).
+  - destruct v; simpl in *; inv H1.
+    exact (set_memory_correct IHfromADT H0).
+Qed.
+
 Theorem allocations_have_size : forall r : Rep HeapSpec, fromADT _ r ->
-  forall addr len, Ensembles.In _ (fst r) (addr, len) -> 0 < len.
+  forall addr len data,
+    Ensembles.In _ r {| memAddr := addr
+                      ; memSize := len
+                      ; memData := data |} -> 0 < len.
 Proof.
   intros.
+  generalize dependent data.
   generalize dependent len.
   generalize dependent addr.
   ADT induction r.
   - inversion H0.
   - simplify_ensembles.
-      exact (IHfromADT _ _ H2).
+      exact (IHfromADT _ _ _ H2).
     destruct x; trivial.
-  - revert H0'.
-    simplify_ensembles; intros;
-    inv H0'; simplify_ensembles.
-      exact (IHfromADT _ _ H2).
-    exact (IHfromADT _ _ H1).
-  - revert H0'.
-    simplify_ensembles;
-    destruct x0; simpl;
-    unfold IfDec_Then_Else; simpl.
-      destruct (x0 <=? n);
-      simplify_ensembles; simpl in *;
-      subst; trivial.
-        exact (IHfromADT _ _ H2).
-      destruct x0;
-      simplify_ensembles; simpl in *;
-      inv H3; inv H1; inv H3; trivial.
-        exact (IHfromADT _ _ H1).
-      exact (IHfromADT _ _ H1).
-    inv H3; inv H1.
-      exact (IHfromADT _ _ H3).
-    inv H3.
-    assumption.
-  - revert H0'.
-    destruct v; simpl; intros;
-    inv H0'; simpl in *;
-    exact (IHfromADT _ _ H1).
+  - simplify_ensembles; intros.
+    exact (IHfromADT _ _ _ H0).
+  - destruct x0; simpl in *.
+    unfold fit_to_length, shift_address, IfDec_Then_Else in H1; simpl in H1.
+    simplify_ensembles; simpl in *.
+    destruct (x1 =? (if x =? memAddr x3 then x1 else memAddr x3)); inv H4.
+      assumption.
+    apply (@IHfromADT (memAddr x3) (memSize x3) (memData x3)).
+    destruct x3.
+    exact H1.
+  - unfold set_address, IfDec_Then_Else in H0; simpl in H0.
+    simplify_ensembles.
+    destruct ((memAddr x1 <=? x) && (x <? memAddr x1 + memSize x1))%bool;
+    inv H1; simpl in *; inv H2.
+      apply (@IHfromADT (memAddr x1) (memSize x1) (memData x1)).
+      destruct x1.
+      exact H0.
+    exact (IHfromADT _ _ _ H0).
+  - destruct x1; simpl in *.
+    unfold copy_memory, IfDec_Then_Else in H0; simpl in H0.
+    simplify_ensembles.
+    destruct ((memAddr x2 <=? x0) &&
+              (x0 <? memAddr x2 + memSize x2) &&
+              (x0 + x1 <=? memSize x2))%bool;
+    simplify_ensembles.
+      destruct ((memAddr x3 <=? x) &&
+                (x <? memAddr x3 + memSize x3) &&
+                (x + x1 <=? memSize x3))%bool;
+      inv H3; simpl in *; inv H2.
+        apply (@IHfromADT (memAddr x2) (memSize x2) (memData x2)).
+        destruct x2.
+        exact H0.
+      exact (IHfromADT _ _ _ H0).
+    inv H1; simpl in *; inv H2.
+    exact (IHfromADT _ _ _ H0).
+  - destruct x0; simpl in *.
+    unfold set_memory, IfDec_Then_Else in H0; simpl in H0.
+    simplify_ensembles.
+    destruct ((memAddr x2 <=? x) &&
+              (x <? memAddr x2 + memSize x2) &&
+              (x + x0 <=? memSize x2))%bool;
+    inv H1; simpl in *; inv H2.
+      apply (@IHfromADT (memAddr x2) (memSize x2) (memData x2)).
+      destruct x2.
+      exact H0.
+    exact (IHfromADT _ _ _ H0).
 Qed.
 
 Theorem allocations_unique : forall r : Rep HeapSpec, fromADT _ r ->
-  forall addr len1 len2,
-    Ensembles.In _ (fst r) (addr, len1) /\ Ensembles.In _ (fst r) (addr, len2)
-      -> len1 = len2.
+  forall addr len1 data1 len2 data2,
+       Ensembles.In _ r {| memAddr := addr
+                         ; memSize := len1
+                         ; memData := data1 |}
+    -> Ensembles.In _ r {| memAddr := addr
+                         ; memSize := len2
+                         ; memData := data2 |}
+    -> len1 = len2 /\ data1 = data2.
+Proof.
+  intros.
+  generalize dependent data2.
+  generalize dependent len2.
+  generalize dependent data1.
+  generalize dependent len1.
+  ADT induction r.
+  - inversion H0.
+  - destruct x; simpl in *.
+    simplify_ensembles;
+    first [ exact (proj1 (IHfromADT _ _ H2 _ _ H3))
+          | exact (proj2 (IHfromADT _ _ H2 _ _ H3))
+          | specialize (H0 _ _ _ H3);
+            apply (allocations_have_size H) in H3;
+            contradiction (overlaps_irr addr l H3)
+          | specialize (H0 _ _ _ H2);
+            apply (allocations_have_size H) in H2;
+            contradiction (overlaps_irr addr l H2) ].
+  - simplify_ensembles;
+    first [ exact (proj1 (IHfromADT _ _ H2 _ _ H0))
+          | exact (proj2 (IHfromADT _ _ H2 _ _ H0)) ].
+  - admit.
+  - admit.
+  - admit.
+  - admit.
 Admitted.
 
 Theorem allocations_no_overlap : forall r : Rep HeapSpec, fromADT _ r ->
-  forall addr1 len1 addr2 len2,
-    Ensembles.In _ (fst r) (addr1, len1) /\ Ensembles.In _ (fst r) (addr2, len2)
-      -> ~ overlaps addr1 len1 addr2 len2.
-Admitted.
-
-Theorem assignments_unique : forall r : Rep HeapSpec, fromADT _ r ->
-  forall idx val1 val2,
-    Ensembles.In _ (snd r) (idx, val1) /\ Ensembles.In _ (snd r) (idx, val2)
-      -> val1 = val2.
-Admitted.
-
-Theorem assignments_correct : forall r : Rep HeapSpec, fromADT _ r ->
-  forall i v, Ensembles.In _ (snd r) (i, v)
-    -> exists a l, Ensembles.In _ (fst r) (a, l) /\ within a l i.
+  forall addr1 len1 data1 addr2 len2 data2,
+       Ensembles.In _ r {| memAddr := addr1
+                         ; memSize := len1
+                         ; memData := data1 |}
+    -> Ensembles.In _ r {| memAddr := addr2
+                         ; memSize := len2
+                         ; memData := data2 |}
+    -> addr1 <> addr2
+    -> ~ overlaps addr1 len1 addr2 len2.
+Proof.
+  intros.
+  generalize dependent data2.
+  generalize dependent len2.
+  generalize dependent addr2.
+  generalize dependent data1.
+  generalize dependent len1.
+  generalize dependent addr1.
+  ADT induction r.
+  - inversion H0.
+  - simplify_ensembles.
+    + exact (IHfromADT _ _ _ H3 _ H2 _ _ H4).
+    + exact (H0 _ _ _ H4).
+    + specialize (H0 _ _ _ H3); clear IHfromADT H3.
+      unfold not; intros.
+      apply overlaps_sym in H1.
+      contradiction.
+  - simplify_ensembles.
+    exact (IHfromADT _ _ _ H3 _ H2 _ _ H0).
+  - admit.
+  - admit.
+  - admit.
+  - admit.
 Admitted.
 
 End Heap.
